permutation_definitions.v
@@ -1,0 +1,55 @@
+From Coq Require Export Strings.String.
+From Coq Require Export Lists.List.
+From Coq Require Export Program.Equality.
+From Coq Require Export Bool.DecBool.
+From iris.proofmode Require Export tactics.
+Require Export separation_logic.
+
+Inductive base_event :=
+  | Lock : nat -> base_event
+  | Unlock : nat -> base_event
+  | Join : base_event.
+
+Inductive event :=
+  | Base : base_event -> event
+  | Left : event -> event
+  | Right : event -> event.
+
+Global Instance base_event_eq_dec : EqDecision base_event.
+Proof. solve_decision. Defined.
+
+Global Instance event_eq_dec : EqDecision event.
+Proof. solve_decision. Defined.
+
+Definition trace : Type := list event.
+
+Inductive can_swap : event -> event -> Prop :=
+  | left_right_swap e e' :
+      can_swap (Left e) (Right e')
+  | right_left_swap e e' :
+      can_swap (Right e) (Left e')
+  | left_left_swap e e' :
+      can_swap e e' ->
+      can_swap (Left e) (Left e')
+  | right_right_swap e e' :
+      can_swap e e' ->
+      can_swap (Right e) (Right e').
+
+Inductive perm1 : trace -> trace -> Prop :=
+  | perm1_refl t :
+      perm1 t t
+  | perm1_skip x t t' :
+      perm1 t t' ->
+      perm1 (x :: t) (x :: t')
+  | perm1_swap x y t :
+      can_swap x y ->
+      perm1 (x :: y :: t) (y :: x :: t).
+
+Inductive perm : trace -> trace -> Prop :=
+  | perm_single t t' :
+      perm1 t t' ->
+      perm t t'
+  | perm_trans1 t t' t'' : 
+      perm1 t t' ->
+      perm t' t'' ->
+      perm t t''.
