README.md
@@ -1,0 +1,23 @@
+# Concurrent Incorrectness Separation Logic in Coq
+
+This repository contains the Coq mechanization of my master thesis.
+The mechanization is divided into 7 files.
+
+1. `separation_logic.v`: The basics of separation logic. Also contains the values of both our languages.
+2. `memory_error_definitions.v`: The definitions for chapter 3 in the thesis (memory error language and CISL triples)
+3. `memory_error_theorems.v`: The lemmas for chapter 3 in the thesis (memory error language and CISL triples)
+4. `permutation_definitions.v`: The definitions for permutations (sections 4.2 and 4.3 in the thesis)
+5. `permutation_theorems.v`: The lemmas for permutations (sections 4.2 and 4.3 in the thesis)
+6. `deadlock_definitions.v`: The definitions for chapter 4 in the thesis (section 4.1, 4.4, and 4.5)
+7. `deadlock_theorems.v`: The proof of the soundness theorem of chapter 4 (section 4.6)
+
+## Coq version
+
+This mechanization was done using Coq Platform 2023.03.0 (Coq version 8.17.1~2023.08)  
+It uses some lemmas and definitions from packages that are provided by Coq platform.  
+Specifically, we use:
+
+- stdpp version 1.8.0
+- iris version 4.0.0
+
+This mechanization has been checked to work with the above versions on Windows 10 using the recommended Windows (64 bit) installer of Coq Platform and all default settings.
